src/HOL/Library/Multiset.thy
@@ -3720,8 +3720,8 @@ lemma mset_le_irrefl [elim!]:
 lemma wfP_less_multiset[simp]:
   assumes wfP_less: "wfP ((<) :: ('a :: preorder) \<Rightarrow> 'a \<Rightarrow> bool)"
   shows "wfP ((<) :: 'a multiset \<Rightarrow> 'a multiset \<Rightarrow> bool)"
-  using wfP_multp[OF wfP_less] less_multiset_def
-  by (metis wfPUNIVI wfP_induct)
+  unfolding less_multiset_def
+  using wfP_multp[OF wfP_less] .
 
 
 subsubsection \<open>Strict total-order properties\<close>
